Finish main exp theorem

icing/opt_encScript.sml
@@ -10,6 +10,16 @@ open preamble;
 
 val _ = new_theory "opt_enc";
 
+Triviality exp_size_lemma:
+  (∀f n e l. MEM (f,n,e) l ⇒ exp_size e ≤ exp1_size l) ∧
+  (∀n e l. MEM (n,e) l ⇒ exp_size e ≤ exp3_size l) ∧
+  (∀e l. MEM e l ⇒ exp_size e ≤ exp6_size l)
+Proof
+  rpt conj_tac \\ Induct_on ‘l’ \\ fs []
+  \\ rw [] \\ gvs [astTheory.exp_size_def] \\ res_tac \\ gvs []
+  \\ first_x_assum drule \\ fs []
+QED
+
 Definition gather_constants_exp_def:
   gather_constants_exp (Lit (Word64 w)) = [w] ∧
   gather_constants_exp (FpOptimise sc e) = gather_constants_exp e ∧
@@ -40,29 +50,9 @@ Definition gather_constants_exp_def:
   gather_constants_exp (Lannot e l) =
     (gather_constants_exp e)
 Termination
-  WF_REL_TAC ‘measure (λ e. exp_size e)’ \\ fs[]
-  \\ rpt conj_tac
-  \\ fs[astTheory.exp_size_def]
-  \\ TRY (
-    Induct_on `pes` \\ fs[astTheory.exp_size_def]
-    \\ rpt strip_tac \\ res_tac \\ rveq \\ fs[astTheory.exp_size_def]
-    \\ first_x_assum (qspec_then `e` assume_tac) \\ fs[] \\ NO_TAC
-    )
-  \\ TRY (
-    Induct_on `exps` \\ fs[astTheory.exp_size_def]
-    \\ rpt strip_tac \\ res_tac \\ rveq \\ fs[astTheory.exp_size_def]
-    \\ first_x_assum (qspec_then `op` assume_tac) \\ fs[] \\ NO_TAC
-    )
-  \\ rpt strip_tac
-  \\ fs[astTheory.exp_size_def, astTheory.lit_size_def, char_size_def, astTheory.lop_size_def,
-        fpValTreeTheory.fp_opt_size_def]
-  \\ ‘∀ x l. MEM x l ⇒ exp_size x ≤ exp6_size l’ by (
-    rpt strip_tac
-    \\ Induct_on ‘l’ \\ fs[]
-    \\ rpt strip_tac
-    \\ fs[astTheory.exp_size_def]
-    )
-  \\ pop_assum imp_res_tac \\ fs[]
+  WF_REL_TAC ‘measure (λ e. exp_size e)’
+  \\ rw [astTheory.exp_size_def]
+  \\ imp_res_tac exp_size_lemma \\ gvs []
 End
 
 Definition gather_used_identifiers_pat_def:
@@ -92,6 +82,8 @@ Termination
   \\ pop_assum imp_res_tac \\ fs[]
 End
 
+
+
 Definition gather_used_identifiers_exp_def:
   gather_used_identifiers_exp (FpOptimise sc e) =
     gather_used_identifiers_exp e ∧
@@ -103,7 +95,7 @@ Definition gather_used_identifiers_exp_def:
   gather_used_identifiers_exp (Raise e) = gather_used_identifiers_exp e ∧
   gather_used_identifiers_exp (Handle e pes) =
     (gather_used_identifiers_exp e) ++
-    (FLAT (MAP (λ (p,e). (gather_used_identifiers_pat p) ++
+    (FLAT (MAP (λ (p,e). pat_bindings p [] ++
                          (gather_used_identifiers_exp e)) pes)) ∧
   gather_used_identifiers_exp (Con mod exps) =
     FLAT (MAP gather_used_identifiers_exp exps) ∧
@@ -117,7 +109,7 @@ Definition gather_used_identifiers_exp_def:
     (gather_used_identifiers_exp e3) ∧
   gather_used_identifiers_exp (Mat e pes) =
     (gather_used_identifiers_exp e) ++
-    FLAT ((MAP (λ (p,e). (gather_used_identifiers_pat p) ++
+    FLAT ((MAP (λ (p,e). pat_bindings p [] ++
                          gather_used_identifiers_exp e) pes)) ∧
   gather_used_identifiers_exp (Let so e1 e2) =
     (let expression_identifiers =
@@ -126,35 +118,59 @@ Definition gather_used_identifiers_exp_def:
        | NONE => expression_identifiers
        | SOME n => n::expression_identifiers) ∧
   gather_used_identifiers_exp (Letrec ses e) =
-    FLAT (MAP (λ (n, p, _). [n; p]) ses) ++ (gather_used_identifiers_exp e) ∧
+    FLAT (MAP (λ (n, p, e). n :: p :: gather_used_identifiers_exp e) ses) ++
+    (gather_used_identifiers_exp e) ∧
   gather_used_identifiers_exp (Tannot e t) =
     (gather_used_identifiers_exp e) ∧
   gather_used_identifiers_exp (Lannot e l) =
     (gather_used_identifiers_exp e)
 Termination
-  WF_REL_TAC ‘measure (λ e. exp_size e)’ \\ fs[]
-  \\ rpt conj_tac
-  \\ fs[astTheory.exp_size_def]
-  \\ TRY (
-    Induct_on `pes` \\ fs[astTheory.exp_size_def]
-    \\ rpt strip_tac \\ res_tac \\ rveq \\ fs[astTheory.exp_size_def]
-    \\ first_x_assum (qspec_then `e` assume_tac) \\ fs[] \\ NO_TAC
-    )
-  \\ TRY (
-    Induct_on `exps` \\ fs[astTheory.exp_size_def]
-    \\ rpt strip_tac \\ res_tac \\ rveq \\ fs[astTheory.exp_size_def]
-    \\ first_x_assum (qspec_then `op` assume_tac) \\ fs[] \\ NO_TAC
-    )
-  \\ rpt strip_tac
-  \\ fs[astTheory.exp_size_def, astTheory.lit_size_def, char_size_def, astTheory.lop_size_def,
-        fpValTreeTheory.fp_opt_size_def]
-  \\ ‘∀ x l. MEM x l ⇒ exp_size x ≤ exp6_size l’ by (
-    rpt strip_tac
-    \\ Induct_on ‘l’ \\ fs[]
-    \\ rpt strip_tac
-    \\ fs[astTheory.exp_size_def]
-    )
-  \\ pop_assum imp_res_tac \\ fs[]
+  WF_REL_TAC ‘measure (λ e. exp_size e)’
+  \\ rw [astTheory.exp_size_def]
+  \\ imp_res_tac exp_size_lemma \\ gvs []
+End
+
+(**
+  Walk over an AST and replace constants by variables that globally allocate
+  their value
+**)
+Definition replace_constants_exp_def:
+  replace_constants_exp al (Lit (Word64 w)) =
+    (case (ALOOKUP al w) of
+    | NONE => Lit (Word64 w)
+    | SOME v => (Var (Short v))) ∧
+  replace_constants_exp al (FpOptimise sc e) =
+    FpOptimise sc (replace_constants_exp al e) ∧
+  replace_constants_exp al (Lit l) = (Lit l) ∧
+  replace_constants_exp al (Var x) = (Var x) ∧
+  replace_constants_exp al (Raise e) = Raise (replace_constants_exp al e) ∧
+  replace_constants_exp al (Handle e pes) =
+    Handle (replace_constants_exp al e)
+           (MAP (λ (p,e). (p, replace_constants_exp al e)) pes) ∧
+  replace_constants_exp al (Con mod exps) =
+    Con mod (MAP (replace_constants_exp al) exps) ∧
+  replace_constants_exp al (Fun s e) = Fun s (replace_constants_exp al e) ∧
+  replace_constants_exp al (App op exps) =
+    App op (MAP (replace_constants_exp al) exps) ∧
+  replace_constants_exp al (Log lop e2 e3) =
+    Log lop (replace_constants_exp al e2) (replace_constants_exp al e3) ∧
+  replace_constants_exp al (If e1 e2 e3) =
+    If (replace_constants_exp al e1) (replace_constants_exp al e2) (replace_constants_exp al e3) ∧
+  replace_constants_exp al (Mat e pes) =
+    Mat (replace_constants_exp al e) ((MAP (λ (p,e). (p, replace_constants_exp al e)) pes)) ∧
+  replace_constants_exp al (Let so e1 e2) =
+    Let so (replace_constants_exp al e1) (replace_constants_exp al e2) ∧
+  replace_constants_exp al (Letrec ses e) =
+    Letrec (MAP (λ(f,n,e). (f,n,replace_constants_exp al e)) ses)
+      (replace_constants_exp al e) ∧
+  replace_constants_exp al (Tannot e t) =
+    Tannot (replace_constants_exp al e) t ∧
+  replace_constants_exp al (Lannot e l) =
+    Lannot (replace_constants_exp al e) l
+Termination
+  WF_REL_TAC ‘measure (λ (al, e). exp_size e)’
+  \\ rw [astTheory.exp_size_def]
+  \\ imp_res_tac exp_size_lemma \\ gvs []
 End
 
 Inductive v_rel:
@@ -233,6 +249,13 @@ Definition res_rel_def[simp]:
   res_rel _ _ = F
 End
 
+Definition res1_rel_def[simp]:
+  res1_rel (Rval x) (Rval y) = v_rel x y ∧
+  res1_rel (Rerr (Rraise v)) (Rerr (Rraise w)) = v_rel v w ∧
+  res1_rel (Rerr (Rabort a)) (Rerr (Rabort b)) = (a = b) ∧
+  res1_rel _ _ = F
+End
+
 Definition ref_rel_def[simp]:
   ref_rel (Refv v) (Refv w) = v_rel v w ∧
   ref_rel (Varray vs) (Varray ws) = LIST_REL v_rel vs ws ∧
@@ -247,7 +270,7 @@ Definition state_rel_def:
     t.next_type_stamp = s.next_type_stamp ∧
     t.next_exn_stamp = s.next_exn_stamp ∧
     t.fp_state = s.fp_state ∧
-    LIST_REL ref_rel t.refs s.refs
+    LIST_REL ref_rel s.refs t.refs
 End
 
 Theorem do_opapp_SOME_IMP:
@@ -345,8 +368,74 @@ Proof
 QED
 
 Theorem v_rel_do_fpoptimise:
-  LIST_REL v_rel xs ys ⇒
-  LIST_REL v_rel (do_fpoptimise annot xs) (do_fpoptimise annot ys)
+  ∀annot xs ys.
+    LIST_REL v_rel xs ys ⇒
+    LIST_REL v_rel (do_fpoptimise annot xs) (do_fpoptimise annot ys)
+Proof
+  ho_match_mp_tac do_fpoptimise_ind \\ rpt strip_tac
+  \\ gvs [do_fpoptimise_def]
+  \\ TRY (first_assum $ irule_at (Pos last) \\ fs [])
+  \\ fs [PULL_EXISTS]
+  \\ first_x_assum drule_all
+  \\ first_x_assum drule_all
+  \\ metis_tac [LIST_REL_APPEND]
+QED
+
+Definition match_rel_def[simp]:
+  match_rel No_match No_match = T ∧
+  match_rel Match_type_error Match_type_error = T ∧
+  match_rel (Match e1) (Match e2) =
+    LIST_REL (λ(s1,x1) (s2,x2). s1 = (s2:string) ∧ v_rel x1 x2) e1 e2 ∧
+  match_rel _ _ = F
+End
+
+Theorem pmatch_thm:
+  (∀envc refs1 p v xs v1 ys refs2.
+     LIST_REL ref_rel refs2 refs1 ∧
+     v_rel v v1 ∧ match_rel (Match xs) (Match ys) ⇒
+     match_rel (pmatch envc refs1 p v xs)
+               (pmatch envc refs2 p v1 ys)) ∧
+  (∀envc refs1 ps vs xs vs1 ys refs2.
+     LIST_REL ref_rel refs2 refs1 ∧
+     LIST_REL v_rel vs vs1 ∧ match_rel (Match xs) (Match ys) ⇒
+     match_rel (pmatch_list envc refs1 ps vs xs)
+               (pmatch_list envc refs2 ps vs1 ys))
+Proof
+  cheat
+QED
+
+Theorem pmatch_pat_bindings:
+  pmatch envc refs p v [] = Match a ⇒
+  set (MAP FST a) SUBSET set (pat_bindings p [])
+Proof
+  cheat
+QED
+
+Theorem v_rel_Boolv_id:
+  ∀b. v_rel (Boolv b) (Boolv b)
+Proof
+  Cases \\ fs [Boolv_def]
+QED
+
+Theorem res1_rel_Rerr[simp]:
+  res1_rel (Rerr e) (Rerr e') = res_rel (Rerr e) (Rerr e')
+Proof
+  Cases_on ‘e’ \\ Cases_on ‘e'’ \\ fs []
+QED
+
+Theorem v_rel_Boolv:
+  v_rel v' v ⇒ (v' = Boolv b ⇔ v = Boolv b)
+Proof
+  Cases_on ‘b’ \\ Cases_on ‘v'’ \\ Cases_on ‘v’ \\ fs [Boolv_def]
+  \\ rw [] \\ eq_tac \\ rw [] \\ gvs []
+QED
+
+Theorem do_app_thm:
+  ∀op a1 a2 refs1 refs2 ffi.
+    LIST_REL v_rel a1 a2 ∧ LIST_REL ref_rel refs1 refs2 ⇒
+    OPTREL (λ((r1,f1),v1) ((r2,f2),v2).
+             f1 = f2 ∧ res1_rel v1 v2 ∧ LIST_REL ref_rel r1 r2)
+           (do_app (refs1,ffi) op a1) (do_app (refs2,ffi) op a2)
 Proof
   cheat
 QED
@@ -362,6 +451,8 @@ Theorem replace_constants_exp_thm:
         state_rel s1 t1 ∧ res_rel res res1) ∧
   (∀(s:'ffi state) env v pes err v1 err1 s1 res t env1 al.
      DISJOINT (set (FLAT (MAP (gather_used_identifiers_exp o SND) pes)))
+              (set (MAP SND al)) ∧
+     DISJOINT (set (FLAT (MAP (λ(p,e). pat_bindings p []) pes)))
               (set (MAP SND al)) ∧
      evaluate_match s env v pes err = (s1,res) ∧
      state_rel s t ∧ env_rel env env1 al ∧ v_rel v v1 ∧ v_rel err err1 ⇒
@@ -509,9 +600,77 @@ Proof
         \\ once_rewrite_tac [find_recfun_def] \\ gvs []
         \\ gvs [FORALL_PROD] \\ rw [])
       \\ irule env_rel_build_rec_env \\ fs [])
-    \\ cheat (* long and boring *))
-  THEN1 (rename [‘Log’] \\ cheat)
-  THEN1 (rename [‘If’] \\ cheat)
+    \\ fs [replace_constants_exp_def]
+    \\ ‘getOpClass op ≠ FunApp’ by
+      (Cases_on ‘op’ \\ fs [astTheory.getOpClass_def])
+    \\ gvs []
+    \\ fs [evaluate_def,CaseEq"prod",gather_used_identifiers_exp_def]
+    \\ rpt $ pop_assum mp_tac
+    \\ CONV_TAC (DEPTH_CONV ETA_CONV) \\ rpt strip_tac \\ gvs []
+    \\ last_x_assum $ drule_at (Pos last)
+    \\ disch_then $ drule_at (Pos last)
+    \\ impl_tac THEN1 fs [IN_DISJOINT,MEM_FLAT,MEM_MAP]
+    \\ strip_tac \\ gvs [PULL_EXISTS]
+    \\ rename [‘res_rel res0 res1’]
+    \\ Cases_on ‘res0’ \\ Cases_on ‘res1’ \\ gvs [MAP_REVERSE]
+    \\ qspecl_then [‘op’,‘REVERSE a’,‘REVERSE a'’,‘st'.refs’,‘t1.refs’,‘t1.ffi’]
+          mp_tac do_app_thm
+    \\ impl_tac
+    THEN1 (fs [LIST_REL_REVERSE_EQ] \\ fs [state_rel_def])
+    \\ rename [‘state_rel s1 t1’]
+    \\ ‘s1.ffi = t1.ffi’ by fs [state_rel_def]
+    \\ Cases_on ‘getOpClass op = Simple’ \\ gvs []
+    THEN1
+     (rw [] \\ gvs [AllCaseEqs()]
+      \\ Cases_on ‘do_app (t1.refs,t1.ffi) op (REVERSE a')’ \\ fs []
+      \\ PairCases_on ‘x’ \\ gvs []
+      \\ fs [state_rel_def]
+      \\ rename [‘res_rel (list_result g1) (list_result g2)’]
+      \\ Cases_on ‘g1’ \\ Cases_on ‘g2’ \\ gvs []
+      \\ Cases_on ‘e’ \\ Cases_on ‘e'’ \\ gvs [])
+    \\ Cases_on ‘getOpClass op = Reals’ \\ gvs []
+    THEN1
+     (rw [] \\ gvs [AllCaseEqs()]
+      \\ Cases_on ‘do_app (t1.refs,t1.ffi) op (REVERSE a')’ \\ fs []
+      \\ TRY (gvs [state_rel_def,shift_fp_opts_def] \\ NO_TAC)
+      \\ PairCases_on ‘x’ \\ gvs []
+      \\ fs [state_rel_def]
+      \\ rename [‘res_rel (list_result g1) (list_result g2)’]
+      \\ Cases_on ‘g1’ \\ Cases_on ‘g2’ \\ gvs []
+      \\ Cases_on ‘e’ \\ Cases_on ‘e'’ \\ gvs [])
+    \\ ‘getOpClass op = Icing’ by (Cases_on ‘getOpClass op’ \\ fs [])
+    \\ gvs [AllCaseEqs()]
+    \\ Cases_on ‘do_app (t1.refs,t1.ffi) op (REVERSE a')’ \\ fs []
+    \\ PairCases_on ‘x’ \\ gvs []
+    \\ fs [state_rel_def,shift_fp_opts_def]
+    \\ rw [] \\ gvs []
+    \\ TRY (Cases_on ‘r’ \\ Cases_on ‘x2’) \\ fs [do_fprw_def]
+    \\ TRY (Cases_on ‘a''’ \\ Cases_on ‘a'''’) \\ fs [v_rel_Boolv]
+    \\ every_case_tac \\ fs [v_rel_Boolv_id]
+    \\ metis_tac [])
+  THEN1
+   (rename [‘Log’]
+    \\ gvs [evaluate_def,gather_used_identifiers_exp_def,replace_constants_exp_def]
+    \\ gvs [CaseEq"prod"]
+    \\ first_x_assum drule_all \\ strip_tac \\ gvs []
+    \\ rename [‘res_rel res0 res1’]
+    \\ reverse (Cases_on ‘res0’) \\ Cases_on ‘res1’ \\ gvs []
+    \\ imp_res_tac evaluatePropsTheory.evaluate_sing \\ gvs []
+    \\ gvs [AllCaseEqs()]
+    \\ Cases_on ‘lop’ \\ gvs [do_log_def,AllCaseEqs()]
+    \\ imp_res_tac v_rel_Boolv \\ fs [])
+  THEN1
+   (rename [‘If’]
+    \\ gvs [evaluate_def,gather_used_identifiers_exp_def,replace_constants_exp_def]
+    \\ gvs [CaseEq"prod"]
+    \\ first_x_assum drule_all \\ strip_tac \\ gvs []
+    \\ rename [‘res_rel res0 res1’]
+    \\ reverse (Cases_on ‘res0’) \\ Cases_on ‘res1’ \\ gvs []
+    \\ imp_res_tac evaluatePropsTheory.evaluate_sing \\ gvs []
+    \\ gvs [do_if_def,AllCaseEqs()]
+    \\ imp_res_tac v_rel_Boolv \\ gvs []
+    THEN1 (first_x_assum (qspec_then ‘T’ assume_tac) \\ gvs [])
+    THEN1 (first_x_assum (qspec_then ‘F’ assume_tac) \\ gvs []))
   THEN1
    (rename [‘Mat’]
     \\ gvs [evaluate_def,gather_used_identifiers_exp_def,replace_constants_exp_def]
@@ -531,8 +690,33 @@ Proof
     \\ first_x_assum irule \\ gvs []
     \\ fs [IN_DISJOINT,MEM_FLAT,MEM_MAP,FORALL_PROD,bind_exn_v_def]
     \\ metis_tac [MEM_APPEND])
-  THEN1 (rename [‘Let’] \\ cheat)
-  THEN1 (rename [‘Letrec’] \\ cheat)
+  THEN1
+   (rename [‘Let’]
+    \\ Cases_on ‘xo’
+    \\ gvs [evaluate_def,gather_used_identifiers_exp_def,replace_constants_exp_def]
+    \\ gvs [CaseEq"prod"]
+    \\ first_x_assum drule_all \\ strip_tac \\ gvs []
+    \\ rename [‘res_rel res0 res1’]
+    \\ reverse (Cases_on ‘res0’) \\ Cases_on ‘res1’ \\ gvs []
+    \\ imp_res_tac evaluatePropsTheory.evaluate_sing \\ gvs []
+    \\ gvs [namespaceTheory.nsOptBind_def]
+    \\ first_x_assum irule \\ gvs []
+    \\ irule env_rel_update \\ gvs [])
+  THEN1
+   (rename [‘Letrec’]
+    \\ gvs [evaluate_def,replace_constants_exp_def,
+            gather_used_identifiers_exp_def]
+    \\ gvs [MAP_MAP_o,o_DEF,LAMBDA_PROD,CaseEq"bool"]
+    \\ qmatch_goalsub_abbrev_tac ‘evaluate _ env11’
+    \\ last_x_assum drule
+    \\ disch_then drule
+    \\ disch_then (qspec_then ‘env11’ mp_tac)
+    \\ reverse impl_tac THEN1 (rw [] \\ fs [])
+    \\ unabbrev_all_tac
+    \\ qmatch_goalsub_abbrev_tac ‘MAP ll’
+    \\ ‘ll = (I ## I ## replace_constants_exp al)’ by
+      fs [Abbr‘ll’,FUN_EQ_THM,FORALL_PROD]
+    \\ gvs [] \\ irule env_rel_build_rec_env \\ gvs [])
   THEN1
    (gvs [evaluate_def,replace_constants_exp_def,gather_used_identifiers_exp_def])
   THEN1
@@ -556,7 +740,27 @@ Proof
   THEN1
    (gvs [evaluate_def,replace_constants_exp_def,gather_used_identifiers_exp_def]
     \\ gvs [CaseEq"bool"]
-    \\ cheat)
+    \\ ‘env1.c = env.c’ by fs [env_rel_def] \\ fs []
+    \\ ‘LIST_REL ref_rel t.refs s.refs’ by fs [state_rel_def]
+    \\ drule $ CONJUNCT1 pmatch_thm
+    \\ disch_then $ qspecl_then [‘env.c’,‘p’,‘v’,‘[]’,‘v1’,‘[]’] mp_tac
+    \\ fs [] \\ strip_tac
+    \\ Cases_on ‘pmatch env.c s.refs p v []’
+    \\ Cases_on ‘pmatch env.c t.refs p v1 []’ \\ gvs []
+    \\ last_x_assum drule
+    \\ disch_then drule
+    \\ disch_then irule
+    \\ ‘DISJOINT (set (MAP FST a)) (set (MAP SND al))’ by
+      (imp_res_tac pmatch_pat_bindings
+       \\ fs [IN_DISJOINT,SUBSET_DEF] \\ metis_tac [])
+    \\ pop_assum mp_tac
+    \\ ntac 2 (pop_assum kall_tac)
+    \\ pop_assum mp_tac
+    \\ qid_spec_tac ‘a'’
+    \\ qid_spec_tac ‘a’
+    \\ Induct \\ fs []
+    \\ fs [PULL_EXISTS,FORALL_PROD] \\ rw []
+    \\ irule env_rel_update_lemma \\ fs [])
 QED
 
 val _ = export_theory();
